AwsEncryptionSDK/src/Serialize/V2HeaderBody.dfy
@@ -1,12 +1,8 @@
 // Copyright Amazon.com Inc. or its affiliates. All Rights Reserved.
 // SPDX-License-Identifier: Apache-2.0
 
-include "../../../libraries/src/Collections/Sequences/Seq.dfy"
-include "../../Generated/AwsCryptographicMaterialProviders.dfy"
-include "../../AwsCryptographicMaterialProviders/Client.dfy"
-include "../../StandardLibrary/StandardLibrary.dfy"
-include "../../Util/UTF8.dfy"
-include "./SerializableTypes.dfy"
+include "../../Model/AwsEncryptionSdkTypes.dfy"
+include "SerializableTypes.dfy"
 include "SerializeFunctions.dfy"
 include "HeaderTypes.dfy"
 include "SharedHeaderFunctions.dfy"
@@ -14,11 +10,11 @@ include "EncryptionContext.dfy"
 include "EncryptedDataKeys.dfy"
 
 module V2HeaderBody {
-  import Aws.Crypto
+  import Types = AwsEncryptionSdkTypes
+  import MaterialProviders
   import Seq
   import HeaderTypes
   import opened SharedHeaderFunctions
-  import MaterialProviders.Client
   import opened EncryptedDataKeys
   import opened EncryptionContext
   import opened SerializableTypes
@@ -58,7 +54,7 @@ module V2HeaderBody {
     //# *  Algorithm Suite ID (../data-format/message-header.md#algorithm-
     //# suite-id): MUST correspond to the algorithm suite (../framework/
     //# algorithm-suites.md) used in this behavior
-    + (WriteESDKSuiteId(body.esdkSuiteId)
+    + (WriteESDKSuiteId(body.algorithmSuite)
     //= compliance/client-apis/encrypt.txt#2.6.2
     //# *  Message ID (../data-format/message-header.md#message-id): The
     //# process used to generate this identifier MUST use a good source of
@@ -96,7 +92,8 @@ module V2HeaderBody {
 
   function method {:vcs_split_on_every_assert} ReadV2HeaderBody(
     buffer: ReadableBuffer,
-    maxEdks: Option<posInt64>
+    maxEdks: Option<Types.CountingNumbers>,
+    mpl: MaterialProviders.MaterialProvidersClient
   )
     :(res: ReadCorrect<V2HeaderBody>)
     ensures CorrectlyReadV2HeaderBody(buffer, res)
@@ -104,12 +101,10 @@ module V2HeaderBody {
     var version :- ReadMessageFormatVersion(buffer);
     :- Need(version.data.V2?, Error("Message version must be version 2."));
 
-    var esdkSuiteId :- ReadESDKSuiteId(version.tail);
-    var suiteId := GetAlgorithmSuiteId(esdkSuiteId.data);
-    var suite := Client.SpecificationClient().GetSuite(suiteId);
-    :- Need(suite.commitment.HKDF?, Error("Algorithm suite must support commitment."));
+    var suite :- ReadESDKSuiteId(version.tail, mpl);
+    :- Need(suite.data.commitment.HKDF?, Error("Algorithm suite must support commitment."));
 
-    var messageId :- ReadMessageIdV2(esdkSuiteId.tail);
+    var messageId :- ReadMessageIdV2(suite.tail);
 
     var encryptionContext :- EncryptionContext.ReadAADSection(messageId.tail);
 
@@ -119,11 +114,11 @@ module V2HeaderBody {
 
     var frameLength :- ReadUInt32(contentType.tail);
 
-    var suiteData :- Read(frameLength.tail, suite.commitment.outputKeyLength as nat);
-    assert |suiteData.data| == suite.commitment.outputKeyLength as nat;
+    var suiteData :- Read(frameLength.tail, suite.data.commitment.HKDF.outputKeyLength as nat);
+    assert |suiteData.data| == suite.data.commitment.HKDF.outputKeyLength as nat;
 
     var body:V2HeaderBody := HeaderTypes.V2HeaderBody(
-      esdkSuiteId := esdkSuiteId.data,
+      algorithmSuite := suite.data,
       messageId := messageId.data,
       encryptionContext := encryptionContext.data,
       encryptedDataKeys := encryptedDataKeys.data,
@@ -132,36 +127,23 @@ module V2HeaderBody {
       suiteData := suiteData.data
     );
 
-    assert version.tail.start - buffer.start == 1;
-    assert esdkSuiteId.tail.start - version.tail.start == 2;
-    assert messageId.tail.start - esdkSuiteId.tail.start == 32;
-    assert messageId.tail.start == buffer.start + headerBytesToAADStart;
-
-    assert if IsExpandedAADSection(messageId.tail) then
-      IsV2ExpandedAADSection(buffer)
-    else
-      !IsV2ExpandedAADSection(buffer);
-
-    assert WriteMessageFormatVersion(version.data)
-      + WriteESDKSuiteId(body.esdkSuiteId)
-      + WriteMessageId(body.messageId)
-      <= buffer.bytes[buffer.start..];
-
-    assert if IsV2ExpandedAADSection(buffer) then
-      WriteExpandedAADSection(body.encryptionContext) <= buffer.bytes[messageId.tail.start..]
-    else
-      WriteAADSection(body.encryptionContext) <= buffer.bytes[messageId.tail.start..];
-
-    assert WriteEncryptedDataKeysSection(body.encryptedDataKeys)
-      + WriteContentType(body.contentType)
-      + WriteUint32(body.frameLength)
-      + Write(body.suiteData)
-      <= buffer.bytes[encryptionContext.tail.start..];
-
-    assert if IsV2ExpandedAADSection(buffer) then
-      WriteV2ExpandedAADSectionHeader(body) <= buffer.bytes[buffer.start..]
-    else
-      WriteV2HeaderBody(body) <= buffer.bytes[buffer.start..];
+    assert CorrectlyReadV2HeaderBody(buffer, Success(SuccessfulRead(body, suiteData.tail))) by {
+      if IsV2ExpandedAADSection(buffer) {
+        assert 0 == |body.encryptionContext|;
+        assert messageId.tail.start + 4 == encryptionContext.tail.start;
+        assert WriteV2ExpandedAADSectionHeaderBody(body) <= buffer.bytes[buffer.start..];
+      } else {
+        if 0 < |body.encryptionContext| {
+          HeadersAreTheSameWhenThereIsEncryptionContext(body);
+          assert WriteMessageFormatVersion(HeaderTypes.MessageFormatVersion.V2) <= buffer.bytes[buffer.start..];
+          assert WriteV2ExpandedAADSectionHeaderBody(body) <= buffer.bytes[buffer.start..];
+          assert WriteV2HeaderBody(body) <= buffer.bytes[buffer.start..];
+        } else {
+          assert messageId.tail.start + 2 == encryptionContext.tail.start;
+          assert WriteV2HeaderBody(body) <= buffer.bytes[buffer.start..];
+        }
+      }
+    }
 
     Success(SuccessfulRead(body, suiteData.tail))
   }
@@ -172,7 +154,7 @@ module V2HeaderBody {
   )
   {
     if IsV2ExpandedAADSection(buffer) then
-      CorrectlyRead(buffer, res, WriteV2ExpandedAADSectionHeader)
+      CorrectlyRead(buffer, res, WriteV2ExpandedAADSectionHeaderBody)
     else
       CorrectlyRead(buffer, res, WriteV2HeaderBody)
   }
@@ -190,7 +172,7 @@ module V2HeaderBody {
   // because it is *only* used for correctness.
   // This represents the sub-optimal encoding of AAD
   // where empty AAD is encoded with an extra 2 bytes.
-  function WriteV2ExpandedAADSectionHeader(
+  function WriteV2ExpandedAADSectionHeaderBody(
     body: V2HeaderBody
   )
     :(ret: seq<uint8>)
@@ -200,7 +182,7 @@ module V2HeaderBody {
     // (knowing that (a + b) + c == a + (b + c) ).
     // So manually adding the () helps make it clear.
       WriteMessageFormatVersion(HeaderTypes.MessageFormatVersion.V2)
-    + (WriteESDKSuiteId(body.esdkSuiteId)
+    + (WriteESDKSuiteId(body.algorithmSuite)
     + (WriteMessageId(body.messageId)
     + (WriteExpandedAADSection(body.encryptionContext)
     + (WriteEncryptedDataKeysSection(body.encryptedDataKeys)
@@ -208,4 +190,10 @@ module V2HeaderBody {
     + (WriteUint32(body.frameLength)
     + (Write(body.suiteData))))))))
   }
+
+  lemma HeadersAreTheSameWhenThereIsEncryptionContext(body: V2HeaderBody)
+    requires 0 < |body.encryptionContext|
+    ensures WriteV2ExpandedAADSectionHeaderBody(body) == WriteV2HeaderBody(body)
+  {}
+
 }
