AwsEncryptionSDK/Model/AwsEncryptionSdkTypes.dfy
@@ -1,0 +1,320 @@
+// Copyright Amazon.com Inc. or its affiliates. All Rights Reserved.
+// SPDX-License-Identifier: Apache-2.0
+// Do not modify this file. This file is machine generated, and any changes to it will be overwritten.
+include "../../StandardLibrary/src/Index.dfy"
+ include "../../AwsCryptographicMaterialProviders/src/Index.dfy"
+ include "../../AwsCryptographyPrimitives/src/Index.dfy"
+ module {:extern "Dafny.Aws.EncryptionSdk.Types" } AwsEncryptionSdkTypes
+ {
+ import opened Wrappers
+ import opened StandardLibrary.UInt
+ import opened UTF8
+ import AwsCryptographyMaterialProvidersTypes
+ import AwsCryptographyPrimitivesTypes
+ // Generic helpers for verification of mock/unit tests.
+ datatype DafnyCallEvent<I, O> = DafnyCallEvent(input: I, output: O)
+ 
+ // Begin Generated Types
+ 
+ class IAwsEncryptionSdkClientCallHistory {
+ ghost constructor() {
+ Encrypt := [];
+ Decrypt := [];
+}
+ ghost var Encrypt: seq<DafnyCallEvent<EncryptInput, Result<EncryptOutput, Error>>>
+ ghost var Decrypt: seq<DafnyCallEvent<DecryptInput, Result<DecryptOutput, Error>>>
+}
+ trait {:termination false} IAwsEncryptionSdkClient
+ {
+ // Helper to define any additional modifies/reads clauses.
+ // If your operations need to mutate state,
+ // add it in your constructor function:
+ // Modifies := {your, fields, here, History};
+ // If you do not need to mutate anything:
+ // Modifies := {History};
+ ghost const Modifies: set<object>
+ // For an unassigned const field defined in a trait,
+ // Dafny can only assign a value in the constructor.
+ // This means that for Dafny to reason about this value,
+ // it needs some way to know (an invariant),
+ // about the state of the object.
+ // This builds on the Valid/Repr paradigm
+ // To make this kind requires safe to add
+ // to methods called from unverified code,
+ // the predicate MUST NOT take any arguments.
+ // This means that the correctness of this requires
+ // MUST only be evaluated by the class itself.
+ // If you require any additional mutation,
+ // Then you MUST ensure everything you need in ValidState.
+ // You MUST also ensure ValidState in your constructor.
+ predicate ValidState()
+ ensures ValidState() ==> History in Modifies
+  ghost const History: IAwsEncryptionSdkClientCallHistory
+ predicate EncryptEnsuresPublicly(input: EncryptInput, output: Result<EncryptOutput, Error>)
+ // The public method to be called by library consumers
+ method Encrypt ( input: EncryptInput )
+ returns (output: Result<EncryptOutput, Error>)
+ requires
+ && ValidState() && ( input.materialsManager.Some? ==>
+ && input.materialsManager.value.ValidState()
+ && input.materialsManager.value.Modifies !! {History}
+ ) && ( input.keyring.Some? ==>
+ && input.keyring.value.ValidState()
+ && input.keyring.value.Modifies !! {History}
+ )
+ modifies Modifies - {History} ,
+ (if input.materialsManager.Some? then input.materialsManager.value.Modifies else {}) ,
+ (if input.keyring.Some? then input.keyring.value.Modifies else {}) ,
+ History`Encrypt
+ // Dafny will skip type parameters when generating a default decreases clause.
+ decreases Modifies - {History} ,
+ (if input.materialsManager.Some? then input.materialsManager.value.Modifies else {}) ,
+ (if input.keyring.Some? then input.keyring.value.Modifies else {})
+ ensures
+ && ValidState()
+ ensures EncryptEnsuresPublicly(input, output)
+ ensures History.Encrypt == old(History.Encrypt) + [DafnyCallEvent(input, output)]
+ 
+ predicate DecryptEnsuresPublicly(input: DecryptInput, output: Result<DecryptOutput, Error>)
+ // The public method to be called by library consumers
+ method Decrypt ( input: DecryptInput )
+ returns (output: Result<DecryptOutput, Error>)
+ requires
+ && ValidState() && ( input.materialsManager.Some? ==>
+ && input.materialsManager.value.ValidState()
+ && input.materialsManager.value.Modifies !! {History}
+ ) && ( input.keyring.Some? ==>
+ && input.keyring.value.ValidState()
+ && input.keyring.value.Modifies !! {History}
+ )
+ modifies Modifies - {History} ,
+ (if input.materialsManager.Some? then input.materialsManager.value.Modifies else {}) ,
+ (if input.keyring.Some? then input.keyring.value.Modifies else {}) ,
+ History`Decrypt
+ // Dafny will skip type parameters when generating a default decreases clause.
+ decreases Modifies - {History} ,
+ (if input.materialsManager.Some? then input.materialsManager.value.Modifies else {}) ,
+ (if input.keyring.Some? then input.keyring.value.Modifies else {})
+ ensures
+ && ValidState()
+ ensures DecryptEnsuresPublicly(input, output)
+ ensures History.Decrypt == old(History.Decrypt) + [DafnyCallEvent(input, output)]
+ 
+}
+ datatype AwsEncryptionSdkConfig = | AwsEncryptionSdkConfig (
+ nameonly commitmentPolicy: Option<AwsCryptographyMaterialProvidersTypes.ESDKCommitmentPolicy> ,
+ nameonly maxEncryptedDataKeys: Option<CountingNumbers>
+ )
+ type CountingNumbers = x: int64 | IsValid_CountingNumbers(x) witness *
+ predicate method IsValid_CountingNumbers(x: int64) {
+ ( 1 <= x  )
+}
+ datatype DecryptInput = | DecryptInput (
+ nameonly ciphertext: seq<uint8> ,
+ nameonly materialsManager: Option<AwsCryptographyMaterialProvidersTypes.ICryptographicMaterialsManager> ,
+ nameonly keyring: Option<AwsCryptographyMaterialProvidersTypes.IKeyring>
+ )
+ datatype DecryptOutput = | DecryptOutput (
+ nameonly plaintext: seq<uint8> ,
+ nameonly encryptionContext: AwsCryptographyMaterialProvidersTypes.EncryptionContext ,
+ nameonly algorithmSuiteId: AwsCryptographyMaterialProvidersTypes.ESDKAlgorithmSuiteId
+ )
+ datatype EncryptInput = | EncryptInput (
+ nameonly plaintext: seq<uint8> ,
+ nameonly encryptionContext: Option<AwsCryptographyMaterialProvidersTypes.EncryptionContext> ,
+ nameonly materialsManager: Option<AwsCryptographyMaterialProvidersTypes.ICryptographicMaterialsManager> ,
+ nameonly keyring: Option<AwsCryptographyMaterialProvidersTypes.IKeyring> ,
+ nameonly algorithmSuiteId: Option<AwsCryptographyMaterialProvidersTypes.ESDKAlgorithmSuiteId> ,
+ nameonly frameLength: Option<FrameLength>
+ )
+ datatype EncryptOutput = | EncryptOutput (
+ nameonly ciphertext: seq<uint8> ,
+ nameonly encryptionContext: AwsCryptographyMaterialProvidersTypes.EncryptionContext ,
+ nameonly algorithmSuiteId: AwsCryptographyMaterialProvidersTypes.ESDKAlgorithmSuiteId
+ )
+ type FrameLength = x: int64 | IsValid_FrameLength(x) witness *
+ predicate method IsValid_FrameLength(x: int64) {
+ ( 1 <= x <= 4294967296 )
+}
+ datatype Error =
+ // Local Error structures are listed here
+ | AwsEncryptionSdkException (
+ nameonly message: string
+ )
+ // Any dependent models are listed here
+ | AwsCryptographyMaterialProviders(AwsCryptographyMaterialProviders: AwsCryptographyMaterialProvidersTypes.Error)
+ | AwsCryptographyPrimitives(AwsCryptographyPrimitives: AwsCryptographyPrimitivesTypes.Error)
+ // The Collection error is used to collect several errors together
+ // This is useful when composing OR logic.
+ // Consider the following method:
+ // 
+ // method FN<I, O>(n:I)
+ //   returns (res: Result<O, Types.Error>)
+ //   ensures A(I).Success? ==> res.Success?
+ //   ensures B(I).Success? ==> res.Success?
+ //   ensures A(I).Failure? && B(I).Failure? ==> res.Failure?
+ // 
+ // If either A || B is successful then FN is successful.
+ // And if A && B fail then FN will fail.
+ // But what information should FN transmit back to the caller?
+ // While it may be correct to hide these details from the caller,
+ // this can not be the globally correct option.
+ // Suppose that A and B can be blocked by different ACLs,
+ // and that their representation of I is only eventually consistent.
+ // How can the caller distinguish, at a minimum for logging,
+ // the difference between the four failure modes?
+ // || (!access(A(I)) && !access(B(I)))
+ // || (!exit(A(I)) && !exit(B(I)))
+ // || (!access(A(I)) && !exit(B(I)))
+ // || (!exit(A(I)) && !access(B(I)))
+ | Collection(list: seq<Error>)
+ // The Opaque error, used for native, extern, wrapped or unknown errors
+ | Opaque(obj: object)
+ type OpaqueError = e: Error | e.Opaque? witness *
+}
+ abstract module AbstractAwsEncryptionSdkService
+ {
+ import opened Wrappers
+ import opened StandardLibrary.UInt
+ import opened UTF8
+ import opened Types = AwsEncryptionSdkTypes
+ import Operations : AbstractAwsEncryptionSdkOperations
+ function method DefaultAwsEncryptionSdkConfig(): AwsEncryptionSdkConfig
+ method ESDK(config: AwsEncryptionSdkConfig := DefaultAwsEncryptionSdkConfig())
+ returns (res: Result<ESDKClient, Error>)
+ ensures res.Success? ==> 
+ && fresh(res.value)
+ && fresh(res.value.Modifies)
+ && fresh(res.value.History)
+ && res.value.ValidState()
+ class ESDKClient extends IAwsEncryptionSdkClient
+ {
+ constructor(config: Operations.InternalConfig)
+ requires Operations.ValidInternalConfig?(config)
+ ensures
+ && ValidState()
+ && fresh(History)
+ && this.config == config
+ const config: Operations.InternalConfig
+ predicate ValidState()
+ ensures ValidState() ==>
+ && Operations.ValidInternalConfig?(config)
+ && History !in Operations.ModifiesInternalConfig(config)
+ && Modifies == Operations.ModifiesInternalConfig(config) + {History}
+ predicate EncryptEnsuresPublicly(input: EncryptInput, output: Result<EncryptOutput, Error>)
+ {Operations.EncryptEnsuresPublicly(input, output)}
+ // The public method to be called by library consumers
+ method Encrypt ( input: EncryptInput )
+ returns (output: Result<EncryptOutput, Error>)
+ requires
+ && ValidState() && ( input.materialsManager.Some? ==>
+ && input.materialsManager.value.ValidState()
+ && input.materialsManager.value.Modifies !! {History}
+ ) && ( input.keyring.Some? ==>
+ && input.keyring.value.ValidState()
+ && input.keyring.value.Modifies !! {History}
+ )
+ modifies Modifies - {History} ,
+ (if input.materialsManager.Some? then input.materialsManager.value.Modifies else {}) ,
+ (if input.keyring.Some? then input.keyring.value.Modifies else {}) ,
+ History`Encrypt
+ // Dafny will skip type parameters when generating a default decreases clause.
+ decreases Modifies - {History} ,
+ (if input.materialsManager.Some? then input.materialsManager.value.Modifies else {}) ,
+ (if input.keyring.Some? then input.keyring.value.Modifies else {})
+ ensures
+ && ValidState()
+ ensures EncryptEnsuresPublicly(input, output)
+ ensures History.Encrypt == old(History.Encrypt) + [DafnyCallEvent(input, output)]
+ {
+ output := Operations.Encrypt(config, input);
+ History.Encrypt := History.Encrypt + [DafnyCallEvent(input, output)];
+}
+ 
+ predicate DecryptEnsuresPublicly(input: DecryptInput, output: Result<DecryptOutput, Error>)
+ {Operations.DecryptEnsuresPublicly(input, output)}
+ // The public method to be called by library consumers
+ method Decrypt ( input: DecryptInput )
+ returns (output: Result<DecryptOutput, Error>)
+ requires
+ && ValidState() && ( input.materialsManager.Some? ==>
+ && input.materialsManager.value.ValidState()
+ && input.materialsManager.value.Modifies !! {History}
+ ) && ( input.keyring.Some? ==>
+ && input.keyring.value.ValidState()
+ && input.keyring.value.Modifies !! {History}
+ )
+ modifies Modifies - {History} ,
+ (if input.materialsManager.Some? then input.materialsManager.value.Modifies else {}) ,
+ (if input.keyring.Some? then input.keyring.value.Modifies else {}) ,
+ History`Decrypt
+ // Dafny will skip type parameters when generating a default decreases clause.
+ decreases Modifies - {History} ,
+ (if input.materialsManager.Some? then input.materialsManager.value.Modifies else {}) ,
+ (if input.keyring.Some? then input.keyring.value.Modifies else {})
+ ensures
+ && ValidState()
+ ensures DecryptEnsuresPublicly(input, output)
+ ensures History.Decrypt == old(History.Decrypt) + [DafnyCallEvent(input, output)]
+ {
+ output := Operations.Decrypt(config, input);
+ History.Decrypt := History.Decrypt + [DafnyCallEvent(input, output)];
+}
+ 
+}
+}
+ abstract module AbstractAwsEncryptionSdkOperations {
+ import opened Wrappers
+ import opened StandardLibrary.UInt
+ import opened UTF8
+ import opened Types = AwsEncryptionSdkTypes
+ type InternalConfig
+ predicate ValidInternalConfig?(config: InternalConfig)
+ function ModifiesInternalConfig(config: InternalConfig): set<object>
+ predicate EncryptEnsuresPublicly(input: EncryptInput, output: Result<EncryptOutput, Error>)
+ // The private method to be refined by the library developer
+
+
+ method Encrypt ( config: InternalConfig,  input: EncryptInput )
+ returns (output: Result<EncryptOutput, Error>)
+ requires
+ && ValidInternalConfig?(config) && ( input.materialsManager.Some? ==>
+ && input.materialsManager.value.ValidState()
+ ) && ( input.keyring.Some? ==>
+ && input.keyring.value.ValidState()
+ )
+ modifies ModifiesInternalConfig(config) ,
+ (if input.materialsManager.Some? then input.materialsManager.value.Modifies else {}) ,
+ (if input.keyring.Some? then input.keyring.value.Modifies else {})
+ // Dafny will skip type parameters when generating a default decreases clause.
+ decreases ModifiesInternalConfig(config) ,
+ (if input.materialsManager.Some? then input.materialsManager.value.Modifies else {}) ,
+ (if input.keyring.Some? then input.keyring.value.Modifies else {})
+ ensures
+ && ValidInternalConfig?(config)
+ ensures EncryptEnsuresPublicly(input, output)
+
+
+ predicate DecryptEnsuresPublicly(input: DecryptInput, output: Result<DecryptOutput, Error>)
+ // The private method to be refined by the library developer
+
+
+ method Decrypt ( config: InternalConfig,  input: DecryptInput )
+ returns (output: Result<DecryptOutput, Error>)
+ requires
+ && ValidInternalConfig?(config) && ( input.materialsManager.Some? ==>
+ && input.materialsManager.value.ValidState()
+ ) && ( input.keyring.Some? ==>
+ && input.keyring.value.ValidState()
+ )
+ modifies ModifiesInternalConfig(config) ,
+ (if input.materialsManager.Some? then input.materialsManager.value.Modifies else {}) ,
+ (if input.keyring.Some? then input.keyring.value.Modifies else {})
+ // Dafny will skip type parameters when generating a default decreases clause.
+ decreases ModifiesInternalConfig(config) ,
+ (if input.materialsManager.Some? then input.materialsManager.value.Modifies else {}) ,
+ (if input.keyring.Some? then input.keyring.value.Modifies else {})
+ ensures
+ && ValidInternalConfig?(config)
+ ensures DecryptEnsuresPublicly(input, output)
+}
