AwsEncryptionSDK/src/AwsEncryptionSdkOperations.dfy
@@ -1,0 +1,612 @@
+// Copyright Amazon.com Inc. or its affiliates. All Rights Reserved.
+// SPDX-License-Identifier: Apache-2.0
+
+include "../Model/AwsEncryptionSdkTypes.dfy"
+include "EncryptDecrypt.dfy"
+
+include "KeyDerivation.dfy"
+
+include "Serialize/SerializableTypes.dfy"
+include "Serialize/Header.dfy"
+include "Serialize/HeaderTypes.dfy"
+include "Serialize/V1HeaderBody.dfy"
+include "Serialize/HeaderAuth.dfy"
+include "Serialize/Frames.dfy"
+include "Serialize/SerializeFunctions.dfy"
+include "Serialize/EncryptionContext.dfy"
+
+module AwsEncryptionSdkOperations refines AbstractAwsEncryptionSdkOperations {
+
+  import Aws.Cryptography.Primitives
+  import MPL = AwsCryptographyMaterialProvidersTypes
+  import MaterialProviders
+  import EncryptDecryptHelpers
+
+  import KeyDerivation
+
+  import SerializableTypes
+  import SerializeFunctions
+
+  import MessageBody
+  import Header
+  import HeaderTypes
+  import HeaderAuth
+  import V1HeaderBody
+  import Frames
+  import EncryptionContext
+
+  datatype Config = Config(
+    nameonly crypto: Primitives.AtomicPrimitivesClient,
+    nameonly mpl: MaterialProviders.MaterialProvidersClient,
+    nameonly commitmentPolicy: AwsCryptographyMaterialProvidersTypes.ESDKCommitmentPolicy,
+    nameonly maxEncryptedDataKeys: Option<CountingNumbers>
+  )
+
+  type InternalConfig = Config
+
+  type FrameLength = frameLength : int64 | 0 < frameLength <= 0xFFFF_FFFF witness *
+
+  predicate ValidInternalConfig?(config: InternalConfig)
+  {
+    && config.crypto.ValidState()
+    && config.mpl.ValidState()
+  }
+
+  function ModifiesInternalConfig(config: InternalConfig) : set<object>
+  {
+    config.crypto.Modifies + config.mpl.Modifies
+  }
+
+  predicate EncryptEnsuresPublicly(input: EncryptInput, output: Result<EncryptOutput, Error>)
+  {true}
+
+  method Encrypt ( config: InternalConfig,  input: EncryptInput )
+    returns (output: Result<EncryptOutput, Error>)
+
+    //= compliance/client-apis/encrypt.txt#2.6.1
+    //= type=implication
+    //# If an input algorithm suite (Section 2.4.5) is provided that is not
+    //# supported by the commitment policy (client.md#commitment-policy)
+    //# configured in the client (client.md) encrypt MUST yield an error.
+    //
+    //= compliance/client-apis/client.txt#2.4.2.1
+    //= type=implication
+    //# *  encrypt (encrypt.md) MUST only support algorithm suites that have
+    //# a Key Commitment (../framework/algorithm-suites.md#algorithm-
+    //# suites-encryption-key-derivation-settings) value of False
+    //
+    //= compliance/client-apis/client.txt#2.4.2.2
+    //= type=implication
+    //# *  encrypt (encrypt.md) MUST only support algorithm suites that have
+    //# a Key Commitment (../framework/algorithm-suites.md#algorithm-
+    //# suites-encryption-key-derivation-settings) value of True
+    //
+    //= compliance/client-apis/client.txt#2.4.2.3
+    //= type=implication
+    //# *  encrypt (encrypt.md) MUST only support algorithm suites that have
+    //# a Key Commitment (../framework/algorithm-suites.md#algorithm-
+    //# suites-encryption-key-derivation-settings) value of True
+    ensures
+    (
+      && input.algorithmSuiteId.Some?
+      && config.mpl.ValidateCommitmentPolicyOnEncrypt(MPL.ValidateCommitmentPolicyOnEncryptInput(
+        algorithm := MPL.AlgorithmSuiteId.ESDK(input.algorithmSuiteId.value),
+        commitmentPolicy := MPL.CommitmentPolicy.ESDK(config.commitmentPolicy)
+      )).Failure?
+    )
+    ==>
+      output.Failure?
+
+    //= compliance/client-apis/encrypt.txt#2.4.6
+    //= type=implication
+    //# This value
+    //# MUST be greater than 0 and MUST NOT exceed the value 2^32 - 1.
+    ensures
+      && input.frameLength.Some?
+      && (input.frameLength.value <= 0 || input.frameLength.value > 0xFFFF_FFFF)
+    ==>
+      output.Failure?
+
+    // //= compliance/client-apis/encrypt.txt#2.6.1
+    // //= type=implication
+    // //# If the number of
+    // //# encrypted data keys (../framework/structures.md#encrypted-data-keys)
+    // //# on the encryption materials (../framework/structures.md#encryption-
+    // //# materials) is greater than the maximum number of encrypted data keys
+    // //# (client.md#maximum-number-of-encrypted-data-keys) configured in the
+    // //# client (client.md) encrypt MUST yield an error.
+    // ensures
+    //     && config.maxEncryptedDataKeys.Some?
+    //     && ghostMaterials.Some?
+    //     && |ghostMaterials.value.encryptedDataKeys| > this.maxEncryptedDataKeys.value as int
+    // ==>
+    //     output.Failure?
+  {
+
+    var frameLength : Types.FrameLength :- if input.frameLength.Some? then
+      :- Need(
+      0 < input.frameLength.value <= 0xFFFF_FFFF,
+      Types.AwsEncryptionSdkException(
+      message := "FrameLength must be greater than 0 and less than 2^32")
+      );
+      Success(input.frameLength.value)
+    else
+      Success(EncryptDecryptHelpers.DEFAULT_FRAME_LENGTH);
+
+    :- EncryptDecryptHelpers.ValidateEncryptionContext(input.encryptionContext);
+    var encryptionContext := if input.encryptionContext.Some? then
+      input.encryptionContext.value
+    else
+      map[];
+
+    var cmm :- EncryptDecryptHelpers.CreateCmmFromInput(input.materialsManager, input.keyring);
+
+    //= compliance/client-apis/encrypt.txt#2.4.5
+    //# The algorithm suite (../framework/algorithm-suite.md) that SHOULD be
+    //# used for encryption.
+    var algorithmSuiteId := if input.algorithmSuiteId.Some? then
+      Some(MPL.AlgorithmSuiteId.ESDK(input.algorithmSuiteId.value))
+    else
+      None;
+
+    if algorithmSuiteId.Some? {
+      var _ :- config.mpl
+      .ValidateCommitmentPolicyOnEncrypt(MPL.ValidateCommitmentPolicyOnEncryptInput(
+        algorithm := algorithmSuiteId.value,
+        commitmentPolicy := MPL.CommitmentPolicy.ESDK(config.commitmentPolicy)
+      ))
+      .MapFailure(e => Types.AwsCryptographyMaterialProviders(e));
+    }
+
+    // int64 fits 9 exabytes so we're never going to actually hit this. But if we don't
+    // include this the verifier is not convinced that we can cast the size to int64
+    :- Need(|input.plaintext| < INT64_MAX_LIMIT,
+      Types.AwsEncryptionSdkException(
+      message := "Plaintext exceeds maximum allowed size"));
+
+    var materials :- EncryptDecryptHelpers.GetEncryptionMaterials(
+      cmm,
+      algorithmSuiteId,
+      encryptionContext,
+      //= compliance/client-apis/encrypt.txt#2.6.1
+      //# *  Max Plaintext Length: If the input plaintext (Section 2.4.1) has
+      //# known length, this length MUST be used.
+      |input.plaintext| as int64,
+      config.commitmentPolicy,
+      config.mpl
+    );
+
+    :- EncryptDecryptHelpers.ValidateMaxEncryptedDataKeys(config.maxEncryptedDataKeys, materials.encryptedDataKeys);
+
+    var encryptedDataKeys: SerializableTypes.ESDKEncryptedDataKeys := materials.encryptedDataKeys;
+
+    //= compliance/client-apis/encrypt.txt#2.6.1
+    //# The algorithm suite (../framework/algorithm-suites.md) used in all
+    //# aspects of this operation MUST be the algorithm suite in the
+    //# encryption materials (../framework/structures.md#encryption-
+    //# materials) returned from the Get Encryption Materials (../framework/
+    //# cmm-interface.md#get-encryption-materials) call.
+    var messageId: HeaderTypes.MessageId :- EncryptDecryptHelpers.GenerateMessageId(materials.algorithmSuite, config.crypto);
+
+    var maybeDerivedDataKeys := KeyDerivation.DeriveKeys(
+      messageId, materials.plaintextDataKey.value, materials.algorithmSuite, config.crypto
+    );
+    var derivedDataKeys :- maybeDerivedDataKeys
+      .MapFailure(e => Types.AwsEncryptionSdkException( message := "Failed to derive data keys"));
+
+    var maybeHeader := EncryptDecryptHelpers.BuildHeaderForEncrypt(
+      messageId,
+      materials.algorithmSuite,
+      materials.encryptionContext,
+      encryptedDataKeys,
+      frameLength as uint32,
+      derivedDataKeys,
+      config.crypto
+    );
+
+    :- Need(maybeHeader.Success?, Types.AwsEncryptionSdkException( message := "Failed to build header body"));
+    var header := maybeHeader.value;
+
+    // Encrypt the given plaintext into the framed message
+    var framedMessage :- MessageBody.EncryptMessageBody(
+      input.plaintext,
+      header,
+      derivedDataKeys.dataKey,
+      config.crypto
+    );
+
+    if framedMessage.finalFrame.header.suite.signature.ECDSA? {
+      //= compliance/client-apis/encrypt.txt#2.7.2
+      //# If the algorithm suite (../framework/algorithm-suites.md) contains a
+      //# signature algorithm (../framework/algorithm-suites.md#signature-
+      //# algorithm), this operation MUST calculate a signature over the
+      //# message, and the output encrypted message (Section 2.5.1) MUST
+      //# contain a message footer (../data-format/message-footer.md).
+
+      //= compliance/client-apis/encrypt.txt#2.6
+      //# If the encryption materials gathered (Section 2.6.1) has a
+      //# algorithm suite including a signature algorithm (../framework/
+      //# algorithm-suites.md#signature-algorithm), the encrypt operation
+      //# MUST perform this step.
+
+      //= compliance/data-format/message-footer.txt#2.3
+      //# When an algorithm suite (../framework/algorithm-suites.md) includes a
+      //# signature algorithm (../framework/algorithm-suites.md#signature-
+      //# algorithm), the message (message.md) MUST contain a footer.
+
+      var msg :- EncryptDecryptHelpers.SerializeMessageWithoutSignature(framedMessage, materials.algorithmSuite);
+      var ecdsaParams := framedMessage.finalFrame.header.suite.signature.ECDSA.curve;
+      // TODO: This should just work, but Proof is difficult
+      :- Need(materials.signingKey.Some?,
+      Types.AwsEncryptionSdkException( message := "Missing signing key."));
+
+      //= compliance/client-apis/encrypt.txt#2.7.2
+      //# To calculate a signature, this operation MUST use the signature
+      //# algorithm (../framework/algorithm-suites.md#signature-algorithm)
+      //# specified by the algorithm suite (../framework/algorithm-suites.md),
+      //# with the following input:
+      //#*  the signature key is the signing key (../framework/
+      //#   structures.md#signing-key) in the encryption materials
+      //#   (../framework/structures.md#encryption-materials)
+      //#*  the input to sign is the concatenation of the serialization of the
+      //#   message header (../data-format/message-header.md) and message body
+      //#   (../data-format/message-body.md)
+      var maybeBytes := config.crypto.ECDSASign(
+      Primitives.Types.ECDSASignInput(
+        signatureAlgorithm := ecdsaParams,
+        signingKey := materials.signingKey.value,
+        message := msg
+      )
+      );
+      var bytes :- maybeBytes
+      .MapFailure(e => Types.AwsCryptographyPrimitives(e));
+
+      :- Need(|bytes| < UINT16_LIMIT,
+      Types.AwsEncryptionSdkException(
+        message := "asdfasdf"));
+
+      // TODO
+      // :- Need(|bytes| == ecdsaParams.SignatureLength() as int,
+      //   Types.AwsEncryptionSdkException( message := "Malformed response from Sign()."));
+
+      //= compliance/client-apis/encrypt.txt#2.7.2
+      //# This operation MUST then serialize a message footer with the
+      //# following specifics:
+
+      //= compliance/client-apis/encrypt.txt#2.7.2
+      //# *  Signature Length (../data-format/message-footer.md#signature-
+      //# length): MUST be the length of the output of the calculation
+      //# above.
+
+      //= compliance/client-apis/encrypt.txt#2.7.2
+      //# *  Signature (../data-format/message-footer.md#signature): MUST be
+      //# the output of the calculation above.
+      var signature := UInt16ToSeq(|bytes| as uint16) + bytes;
+
+      //= compliance/client-apis/encrypt.txt#2.7.2
+      //# The encrypted message output by this operation MUST have a message
+      //# footer equal to the message footer calculated in this step.
+      msg := msg + signature;
+      // TODO: Come back and prove this
+      // assert msg == SerializeMessageWithSignature(framedMessage, signature); // Header, frames and signature can be serialized into the stream
+
+      //= compliance/client-apis/encrypt.txt#2.5
+      //# This behavior MUST output the following if the behavior is
+      //# successful:
+      //# *  Encrypted Message (Section 2.5.1)
+      //# *  Encryption Context (Section 2.4.2)
+      //# *  Algorithm Suite (Section 2.4.5)
+      return Success(
+      Types.EncryptOutput(
+        ciphertext := msg,
+        encryptionContext := header.encryptionContext,
+        algorithmSuiteId := header.suite.id.ESDK
+      )
+      );
+    } else {
+      //= compliance/client-apis/encrypt.txt#2.6
+      //# Otherwise the encrypt operation MUST
+      //# NOT perform this step.
+      var msg :- EncryptDecryptHelpers.SerializeMessageWithoutSignature(framedMessage, materials.algorithmSuite);
+      return Success(
+      Types.EncryptOutput(
+        ciphertext := msg,
+        encryptionContext := header.encryptionContext,
+        algorithmSuiteId := header.suite.id.ESDK
+      )
+      );
+    }
+  }
+
+  predicate DecryptEnsuresPublicly(input: DecryptInput, output: Result<DecryptOutput, Error>)
+  {true}
+
+  method Decrypt ( config: InternalConfig,  input: DecryptInput )
+    returns (output: Result<DecryptOutput, Error>)
+    //= compliance/client-apis/decrypt.txt#2.7
+    //= type=TODO
+    //# This operation MUST perform all the above steps unless otherwise
+    //# specified, and it MUST perform them in the above order.
+
+    //= compliance/client-apis/decrypt.txt#2.7.2
+    //= type=implication
+    //# If the parsed algorithm suite ID (../data-format/message-
+    //# header.md#algorithm-suite-id) is not supported by the commitment
+    //# policy (client.md#commitment-policy) configured in the client
+    //# (client.md) decrypt MUST yield an error.
+
+    //= compliance/client-apis/client.txt#2.4.2.1
+    //= type=implication
+    //# *  decrypt (decrypt.md) MUST support all algorithm suites
+    //
+    //= compliance/client-apis/client.txt#2.4.2.2
+    //= type=implication
+    //# *  decrypt (decrypt.md) MUST support all algorithm suites
+    //
+    //= compliance/client-apis/client.txt#2.4.2.3
+    //= type=implication
+    //# *  decrypt (decrypt.md) MUST only support algorithm suites that have
+    //# a Key Commitment (../framework/algorithm-suites.md#algorithm-
+    //# suites-encryption-key-derivation-settings) value of True
+
+    //= compliance/client-apis/decrypt.txt#2.7.2
+    //= type=implication
+    //# If the
+    //# algorithm suite is not supported by the commitment policy
+    //# (client.md#commitment-policy) configured in the client (client.md)
+    //# decrypt MUST yield an error.
+    // TODO :: Consider removing from spec as this is redundant
+    ensures
+    (
+      && var buffer := SerializeFunctions.ReadableBuffer(input.ciphertext, 0);
+      && var headerBody := Header.ReadHeaderBody(buffer, config.maxEncryptedDataKeys, config.mpl);
+      && headerBody.Success?
+      && config.mpl.ValidateCommitmentPolicyOnDecrypt(MPL.ValidateCommitmentPolicyOnDecryptInput(
+        algorithm := headerBody.value.data.algorithmSuite.id,
+        commitmentPolicy := MPL.CommitmentPolicy.ESDK(config.commitmentPolicy)
+      )).Failure?
+    )
+    ==>
+      output.Failure?
+
+    //= compliance/client-apis/decrypt.txt#2.6
+    //= type=implication
+    //# The client MUST return as output to this operation:
+    ensures output.Success?
+    ==>
+      && var buffer := SerializeFunctions.ReadableBuffer(input.ciphertext, 0);
+      && var headerBody := Header.ReadHeaderBody(buffer, config.maxEncryptedDataKeys, config.mpl);
+      && headerBody.Success?
+      // *  Algorithm Suite (Section 2.6.3)
+      && output.value.algorithmSuiteId == headerBody.value.data.algorithmSuite.id.ESDK
+      // *  Encryption Context (Section 2.6.2)
+      && var ec := EncryptionContext.GetEncryptionContext(headerBody.value.data.encryptionContext);
+      && output.value.encryptionContext == ec
+
+    //= compliance/client-apis/decrypt.txt#2.5
+    //= type=implication
+    //# The client MUST require exactly one of the following types of inputs:
+    //#*  Cryptographic Materials Manager (CMM) (../framework/cmm-
+    //#   interface.md)
+    //#*  Keyring (../framework/keyring-interface.md)
+    ensures
+    (
+      || (input.materialsManager.Some? && input.keyring.Some?)
+      || (input.materialsManager.None? && input.keyring.None?)
+    )
+    ==>
+      output.Failure?
+
+  {
+    var cmm :- EncryptDecryptHelpers.CreateCmmFromInput(input.materialsManager, input.keyring);
+
+    //= compliance/client-apis/decrypt.txt#2.7.1
+    //# Given encrypted message bytes, this operation MUST process those
+    //# bytes sequentially, deserializing those bytes according to the
+    //# message format (../data-format/message.md).
+
+    var buffer := SerializeFunctions.ReadableBuffer(input.ciphertext, 0);
+
+    //= compliance/client-apis/decrypt.txt#2.5.1.1
+    //= type=TODO
+    //# To make diagnosing this mistake easier, implementations SHOULD detect
+    //# the first two bytes of the Base64 encoding of any supported message
+    //# versions (../data-format/message-header.md#version-1) and types
+    //# (../data-format/message-header.md#type) and fail with a more specific
+    //# error message.
+
+    var headerBody :- Header
+      .ReadHeaderBody(buffer, config.maxEncryptedDataKeys, config.mpl)
+      .MapFailure(EncryptDecryptHelpers.MapSerializeFailure(": ReadHeaderBody"));
+
+    var rawHeader := headerBody.tail.bytes[buffer.start..headerBody.tail.start];
+
+    var algorithmSuite := headerBody.data.algorithmSuite;
+    //= compliance/client-apis/decrypt.txt#2.7.2
+    //# If the
+    //# algorithm suite is not supported by the commitment policy
+    //# (client.md#commitment-policy) configured in the client (client.md)
+    //# decrypt MUST yield an error.
+    var _ :- config.mpl
+      .ValidateCommitmentPolicyOnDecrypt(MPL.ValidateCommitmentPolicyOnDecryptInput(
+      algorithm := algorithmSuite.id,
+      commitmentPolicy := MPL.CommitmentPolicy.ESDK(config.commitmentPolicy)
+      ))
+      .MapFailure(e => Types.AwsCryptographyMaterialProviders(e));
+
+    //= compliance/client-apis/decrypt.txt#2.5.2
+    //# This CMM MUST obtain the decryption materials (../framework/
+    //# structures.md#decryption-materials) required for decryption.
+
+    //= compliance/client-apis/decrypt.txt#2.5.3
+    //# This default CMM MUST obtain the decryption materials required for
+    //# decryption.
+    // TODO :: Consider removing "Default CMM MUST obtain" from spec.
+    // It is redundent and hard to prove.
+
+    //= compliance/client-apis/decrypt.txt#2.7.2
+    //# This operation MUST obtain this set of decryption materials
+    //# (../framework/structures.md#decryption-materials), by calling Decrypt
+    //# Materials (../framework/cmm-interface.md#decrypt-materials) on a CMM
+    //# (../framework/cmm-interface.md).
+    var decMat :- EncryptDecryptHelpers.GetDecryptionMaterials(
+      cmm,
+      algorithmSuite.id,
+      headerBody.data,
+      config.commitmentPolicy,
+      config.mpl
+    );
+
+    var suite := decMat.algorithmSuite;
+
+    :- Need(suite == algorithmSuite,
+      Types.AwsEncryptionSdkException(
+      message := "Stored header algorithm suite does not match decryption algorithm suite."));
+
+    //= compliance/client-apis/decrypt.txt#2.4.2
+    //# This operation MUST NOT release any unauthenticated plaintext or
+    //# unauthenticated associated data.
+    var headerAuth :- HeaderAuth
+      .ReadHeaderAuthTag(headerBody.tail, suite)
+      .MapFailure(EncryptDecryptHelpers.MapSerializeFailure(": ReadHeaderAuthTag"));
+
+    var maybeDerivedDataKeys := KeyDerivation.DeriveKeys(
+      headerBody.data.messageId, decMat.plaintextDataKey.value, suite, config.crypto
+    );
+    :- Need(maybeDerivedDataKeys.Success?,
+      Types.AwsEncryptionSdkException(
+      message := "Failed to derive data keys"));
+    var derivedDataKeys := maybeDerivedDataKeys.value;
+
+    :- Need(Header.HeaderVersionSupportsCommitment?(suite, headerBody.data),
+      Types.AwsEncryptionSdkException(
+      message := "Invalid commitment values found in header body"));
+    if suite.commitment.HKDF? {
+      var _ :- EncryptDecryptHelpers.ValidateSuiteData(suite, headerBody.data, derivedDataKeys.commitmentKey.value);
+    }
+
+    var maybeHeaderAuth :=
+      //= compliance/client-apis/decrypt.txt#2.7.3
+      //# Once a valid message header is deserialized and decryption materials
+      //# are available, this operation MUST validate the message header body
+      //# (../data-format/message-header.md#header-body) by using the
+      //# authenticated encryption algorithm (../framework/algorithm-
+      //# suites.md#encryption-algorithm) to decrypt with the following inputs:
+      config.crypto.AESDecrypt(Primitives.Types.AESDecryptInput(
+        encAlg := suite.encrypt.AES_GCM,
+        //#*  the cipherkey is the derived data key
+        key := derivedDataKeys.dataKey,
+        //#*  the ciphertext is an empty byte array
+        cipherTxt := [],
+        //#*  the tag is the value serialized in the message header's
+        //#   authentication tag field (../data-format/message-
+        //#   header.md#authentication-tag)
+        authTag := headerAuth.data.headerAuthTag,
+        //#*  the IV is the value serialized in the message header's IV field
+        //#   (../data-format/message-header#iv).
+        iv := headerAuth.data.headerIv,
+        //#*  the AAD is the serialized message header body (../data-format/
+        //#   message-header.md#header-body).
+        aad := rawHeader
+      ));
+    //= compliance/client-apis/decrypt.txt#2.7.3
+    //# If this tag verification fails, this operation MUST immediately halt
+    //# and fail.
+    var _ :- maybeHeaderAuth
+      .MapFailure(e => Types.AwsCryptographyPrimitives(e));
+    assert {:split_here} true;
+
+    var receivedEncryptionContext := EncryptionContext.GetEncryptionContext(
+      headerBody.data.encryptionContext
+    );
+    :- Need(
+      SerializableTypes.IsESDKEncryptionContext(receivedEncryptionContext),
+      Types.AwsEncryptionSdkException(
+        message := "Received invalid encryption context")
+    );
+
+    var header := Header.HeaderInfo(
+      body := headerBody.data,
+      rawHeader := rawHeader,
+      encryptionContext := receivedEncryptionContext,
+      suite := suite,
+      headerAuth := headerAuth.data
+    );
+
+    assert {:split_here} true;
+
+    assert Header.HeaderAuth?(suite, headerAuth.data);
+    assert Header.IsHeader(header);
+
+    var key := derivedDataKeys.dataKey;
+    var plaintext: seq<uint8>;
+
+    var messageBodyTail: SerializeFunctions.ReadableBuffer;
+
+    //= compliance/client-apis/decrypt.txt#2.7.4
+    //# Once the message header is successfully parsed, the next sequential
+    //# bytes MUST be deserialized according to the message body spec
+    //# (../data-format/message-body.md).
+
+    //= compliance/client-apis/decrypt.txt#2.7.4
+    //# The content type (../data-format/message-header.md#content-type)
+    //# field parsed from the message header above determines whether these
+    //# bytes MUST be deserialized as framed data (../data-format/message-
+    //# body.md#framed-data) or un-framed data (../data-format/message-
+    //# body.md#un-framed-data).
+    match header.body.contentType {
+      case NonFramed =>
+        //= compliance/client-apis/decrypt.txt#2.7.4
+        //# If this decryption fails, this operation MUST immediately halt and
+        //# fail.
+        var decryptRes :- EncryptDecryptHelpers.ReadAndDecryptNonFramedMessageBody(headerAuth.tail, header, key, config.crypto);
+        plaintext := decryptRes.0;
+        messageBodyTail := decryptRes.1;
+
+      case Framed =>
+        //= compliance/client-apis/decrypt.txt#2.7.4
+        //# If this decryption fails, this operation MUST immediately halt and
+        //# fail.
+        var decryptRes :- EncryptDecryptHelpers.ReadAndDecryptFramedMessageBody(headerAuth.tail, header, key, config.crypto);
+        plaintext := decryptRes.0;
+        messageBodyTail := decryptRes.1;
+    }
+
+    assert {:split_here} true;
+
+    //= compliance/client-apis/decrypt.txt#2.7.5
+    //# If this verification is not successful, this operation MUST
+    //# immediately halt and fail.
+    var signature :- EncryptDecryptHelpers.VerifySignature(
+      messageBodyTail,
+      messageBodyTail.bytes[buffer.start..messageBodyTail.start],
+      decMat,
+      config.crypto
+    );
+
+    :- Need(signature.start == |signature.bytes|,
+      Types.AwsEncryptionSdkException(
+      message := "Data after message footer."));
+
+    //= compliance/client-apis/decrypt.txt#2.7.1
+    //# Until the header is verified (Section 2.7.3), this operation MUST NOT
+    //# release any parsed information from the header.
+    // Note that the header is verified above
+
+    //= compliance/client-apis/decrypt.txt#2.7.4
+    //# This operation MUST NOT release any unauthenticated plaintext.
+
+    //= compliance/client-apis/decrypt.txt#2.7
+    //# If the input encrypted message is not being streamed (streaming.md)
+    //# to this operation, all output MUST NOT be released until after these
+    //# steps complete successfully.
+    return Success(
+      Types.DecryptOutput(
+        plaintext := plaintext,
+        encryptionContext := header.encryptionContext,
+        algorithmSuiteId := header.suite.id.ESDK
+      )
+    );
+  }
+
+}
